cfrontend/Type_proof_C.v
@@ -1,0 +1,88 @@
+Require Import String ZArith Coq.FSets.FMapAVL Coq.Structures.OrderedTypeEx FunInd.
+Require Import Coq.FSets.FSetProperties Coq.FSets.FMapFacts FMaps FSetAVL Nat PeanoNat Linking.
+Require Import Coq.Arith.EqNat Coq.ZArith.Int Integers AST Maps Linking Ctypes Smallstep SimplExpr.
+Require Import BeePL_aux BeePL_mem BeeTypes BeePL Csyntax Csem Clight Globalenvs BeePL_Csyntax SimplExpr.
+Require Import Initializersproof Cstrategy BeePL_auxlemmas Coqlib Errors BeePL_values BeePL_sem.
+
+From mathcomp Require Import all_ssreflect. 
+
+Lemma c_eval_expr_type_preservation: forall e cge cvm m e' tr m',
+eval_expr cge cvm m RV e tr m' e' ->
+Csyntax.typeof e = Csyntax.typeof e'.
+Proof.
+move=> e. elim: e=> //=.
+(* val *)
++ move=> v ty cge cvm m e' tr m' he. by inversion he; subst.
+(* var *)
++ move=> x ty cge cvm m e' tr m' he. by inversion he; subst.
+(* field *)
++ move=> e' hin f ty cge cvm m e'' tr m' he. by inversion he; subst.
+(* evalof *)
++ move=> e' hin ty cge cvm m e'' tr m' he. by inversion he; subst.
+(* deref *)
++ move=> e' hin ty cge cvm m e'' tr m' he. by inversion he; subst.
+(* addrof *)
++ move=> e' hin ty cge cvm m e'' tr m' he. by inversion he; subst.
+(* uop *)
++ move=> o e' hin ty cge cvm m e'' tr m' he. by inversion he; subst.
+(* bop *)
++ move=> o e1 hin1 e2 hin2 ty cge cvm m e'' tr m' he. by inversion he; subst.
+(* cast *)
++ move=> e' hin ty cge cvm m e'' tr m' he. by inversion he; subst.
+(* seqand *)
++ move=> e1 hin1 e2 hin2 ty cge cvm m e'' tr m' he. by inversion he; subst.
+(* seqor *)
++ move=> e1 hin1 e2 hin2 ty cge cvm m e'' tr m' he. by inversion he; subst.
+(* condition *)
++ move=> e1 hin e2 hin2 e3 hin3 ty cge cvm m e'' tr m' he. by inversion he; subst.
+(* sizeof *)
++ move=> ty1 ty2 cge cvm m e'' tr m' he. by inversion he; subst.
+(* alignof *)
++ move=> ty1 ty2 cge cvm m e'' tr m' he. by inversion he; subst.
+(* assign *)
++ move=> e1 hin e2 hin' ty cge cvm m e'' tr m' he. by inversion he; subst.
+(* assignop *)
++ move=> op e' hin e1 hin' t1 t2 cge cvm m e'' tr m' he. by inversion he; subst.
+(* postincr *)
++ move=> id e' hin ty cge cvm m e'' tr m' he. by inversion he; subst.
+(* comma *)
++ move=> e1 hin e2 hin' ty cge cvm m e'' tr m' he. inversion he; subst.
+  move: (hin cge cvm m r1' t1 m1 H2)=> ht1. 
+  by move: (hin' cge cvm m1 e'' t2 m' H6)=> ht2; subst.
+(* call *)
++ move=> e1 hin args ty cge cvm m e' tr m' he. by inversion he; subst.
+(* builtin *)
++ move=> ef ts args ty cge cvm m e' tr m' he. by inversion he; subst.
+(* loc *)
++ move=> b ofs bf ty cge cvm m e' tr m' he. by inversion he; subst.
+move=> e1 hin t1 t2 cge cvm m e' tr m' he. by inversion he; subst.
+Qed.
+
+(*Lemma div_c_exec : forall cge cvm m ce1 ce2 tr m' a' v1 v2 zv g g' i' rs t,
+eval_expr cge cvm m RV (hd default_expr (exprlist_list_expr ce2)) tr m' a' ->
+eval_simple_rvalue cge cvm m' a' (trans_bvalue_cvalue v2) ->
+signedness_of_type t = Some Signed ->
+is_zero_val v2 || is_overflow_vals v1 v2 ->
+check_div (Econs ce1 ce2) zv (transBeePL_type t) g = Res rs g' i' ->
+rs = Eval zv (transBeePL_type t).
+Proof.
+move=> cge cvm m ce1 ce2 tr m' a' v1 v2 zv g g' i' rs t he he' hs hv hc.
+rewrite /check_div in hc. case: t hs hc=> //=.
++ move=> [] //=.
+  + move=> sz s a [] hs; subst; rewrite /=.
+    case: sz=> //=. move=> [] h1 h2; subst.*)
+
+
+
+
+
+
+
+
+
+
+
+
+
+
+
